support delete (#16)
* add deleted flag

* fix

* fix

* add delete spec & commutativity

* fix

* fix other than concurrent commutative

* fix sorries

* fix

LeanYjs/Algorithm/Invariant/YjsArray.lean
@@ -6,309 +6,18 @@ import LeanYjs.Order.ItemSetInvariant
 import LeanYjs.Order.Totality
 import LeanYjs.Order.Transitivity
 import LeanYjs.Order.Asymmetry
-import LeanYjs.Algorithm.Integrate
+import LeanYjs.Algorithm.Insert.Basic
+import LeanYjs.Algorithm.Insert.Lemmas
+import LeanYjs.Algorithm.Invariant.Basic
 
 variable {A : Type}
 variable [DecidableEq A]
-
-def ArrSet (arr : List (YjsItem A)) : YjsPtr A -> Prop :=
-  fun a => match a with
-  | YjsPtr.itemPtr item => item ∈ arr
-  | YjsPtr.first => True
-  | YjsPtr.last => True
-
-def ArrSetClosed (arr : List (YjsItem A)) : Prop :=
-  IsClosedItemSet (ArrSet arr)
-
-omit [DecidableEq A] in theorem arr_set_closed_push (arr : List (YjsItem A)) (item : YjsItem A) :
-  ArrSetClosed arr ->
-  ArrSet arr item.origin ->
-  ArrSet arr item.rightOrigin ->
-  ArrSetClosed (item :: arr) := by
-  intros hclosed horigin hright
-  constructor <;> try simp [ArrSet]
-  . intros o r id c hor
-    cases o with
-    | itemPtr item' =>
-      simp
-      cases hor with
-      | inr hitem =>
-        right
-        apply hclosed.closedLeft at hitem
-        assumption
-      | inl heq =>
-        subst heq
-        right
-        assumption
-    | first =>
-      simp
-    | last =>
-      simp
-  . intros o r id c hor
-    cases r with
-    | itemPtr item' =>
-      simp
-      cases hor with
-      | inr hitem =>
-        right
-        apply hclosed.closedRight at hitem
-        assumption
-      | inl heq =>
-        subst heq
-        right
-        assumption
-    | first =>
-      simp
-    | last =>
-      simp
-
-omit [DecidableEq A] in theorem arr_set_item_exists_index (arr arr' : List (YjsItem A)) (item : YjsItem A) :
-  ArrSetClosed arr' ->
-  ArrSet arr item ->
-  (∃ l, l ++ arr = arr') ->
-  ∃ i : Fin arr.length, arr[i] = item := by
-  intros hclosed hitem hsublist
-  induction arr with
-  | nil =>
-    simp [ArrSet] at hitem
-  | cons head arr ih =>
-    simp [ArrSet] at hitem
-    cases hitem with
-    | inl heq =>
-      subst heq
-      have zero_lt_len : 0 < (item :: arr).length := by simp
-      exists Fin.mk 0 zero_lt_len
-    | inr hin =>
-      have hsublist' : ∃ l', l' ++ arr = arr' := by
-        obtain ⟨ l, heq ⟩ := hsublist
-        exists (l ++ [head])
-        rw [List.append_assoc]
-        simp; assumption
-      obtain ⟨ i, hi ⟩ := ih hin hsublist'
-      let i' : Fin ((head :: arr).length) := by
-        simp
-        apply Fin.addNat i 1
-      exists i'
-
-omit [DecidableEq A] in theorem arr_set_closed_exists_index_for_origin :
-  ∀ (arr : List (YjsItem A)) (item : YjsItem A),
-  ArrSetClosed arr ->
-  ArrSet arr item ->
-  item.origin = YjsPtr.first ∨ item.origin = YjsPtr.last ∨ ∃ i : Fin arr.length, arr[i] = item.origin := by
-  intros arr item hclosed hitem
-  obtain ⟨ o, r, id, c ⟩ := item
-  apply hclosed.closedLeft at hitem
-  simp [YjsItem.origin]
-  cases o with
-  | first =>
-    left; simp
-  | last =>
-    right; left; simp
-  | itemPtr o =>
-    right; right
-    obtain ⟨ i, h ⟩ := arr_set_item_exists_index arr arr o hclosed hitem (by exists [])
-    exists i
-    simp
-    assumption
-
-omit [DecidableEq A] in theorem arr_set_closed_exists_index_for_right_origin :
-  ∀ (arr : List (YjsItem A)) (item : YjsItem A),
-  ArrSetClosed arr ->
-  ArrSet arr item ->
-  item.rightOrigin = YjsPtr.first ∨ item.rightOrigin = YjsPtr.last ∨ ∃ i : Fin arr.length, arr[i] = item.rightOrigin := by
-  intros arr item hclosed hitem
-  obtain ⟨ o, r, id, c ⟩ := item
-  apply hclosed.closedRight at hitem
-  simp [YjsItem.rightOrigin]
-  cases r with
-  | first =>
-    left; simp
-  | last =>
-    right; left; simp
-  | itemPtr o =>
-    right; right
-    obtain ⟨ i, h ⟩ := arr_set_item_exists_index arr arr o hclosed hitem (by exists [])
-    exists i
-    simp
-    assumption
-
--- omit [DecidableEq A] in theorem yjs_lt_mono (P Q : ItemSet A) (x y : YjsPtr A) :
---   IsClosedItemSet P ->
---   ItemSetInvariant P ->
---   (∀ a, P a -> Q a) ->
---   YjsLt h x y ->
---   YjsLt h x y := by
---   intros hclosedP hinvP hsubset
---   intros hlt
---   revert hlt x y
---   apply Nat.strongRec' (p := fun h => ∀ x y, YjsLt h x y → YjsLt h x y)
---   intros n ih x y hlt
---   cases hlt with
---   | ltOriginOrder _  _ hlt =>
---     apply YjsLt.ltOriginOrder
---     . assumption
---   | ltConflict _ _ _ hlt =>
---     cases hlt with
---     | ltOriginDiff =>
---       apply YjsLt.ltConflict
---       apply ConflictLt.ltOriginDiff
---       all_goals (apply ih; unfold max4; omega)
---       all_goals (assumption)
---     | ltOriginSame =>
---       apply YjsLt.ltConflict
---       apply ConflictLt.ltOriginSame <;> try assumption
---   | ltOrigin _ _ _ _ _ _ hlt =>
---     apply YjsLt.ltOrigin
---     . cases hlt with
---       | leqSame =>
---         apply YjsLeq.leqSame
---       | leqLt =>
---         apply YjsLeq.leqLt
---         apply ih <;> try assumption
---         omega
---   | ltRightOrigin _ _ _ _ _ _ hlt =>
---     apply YjsLt.ltRightOrigin
---     . cases hlt with
---       | leqSame =>
---         apply YjsLeq.leqSame
---       | leqLt =>
---         apply YjsLeq.leqLt
---         apply ih <;> try assumption
---         omega
-
--- omit [DecidableEq A] in theorem yjs_lt'_mono :
---   ∀ (P Q : ItemSet A) (x y : YjsPtr A),
---   IsClosedItemSet P ->
---   ItemSetInvariant P ->
---   (∀ a, P a -> Q a) ->
---   YjsLt' x y -> YjsLt' x y := by
---   intros P Q x y hclosedP hinvP hsubset hlt
---   obtain ⟨ _, hlt ⟩ := hlt
---   constructor
---   apply yjs_lt_mono P Q x y hclosedP hinvP hsubset hlt
-
--- omit [DecidableEq A] in theorem yjs_leq'_mono :
---   ∀ (P Q : ItemSet A) (x y : YjsPtr A),
---   IsClosedItemSet P ->
---   ItemSetInvariant P ->
---   (∀ a, P a -> Q a) ->
---   YjsLeq' x y -> YjsLeq' x y := by
---   intros P Q x y hclosedP hinvP hsubset hleq
---   obtain ⟨ _, hleq ⟩ := hleq
---   cases hleq with
---   | leqSame =>
---     exists 0
---     apply YjsLeq.leqSame
---   | leqLt =>
---     constructor
---     apply YjsLeq.leqLt
---     apply yjs_lt_mono P Q x y hclosedP hinvP hsubset
---     assumption
-
-theorem ItemSetInvariant.eq_set {A} (P Q : ItemSet A) :
-  IsClosedItemSet P →
-  ItemSetInvariant P →
-  (∀x, P x ↔ Q x) →
-  ItemSetInvariant Q := by
-  intros hPclosed hP hiff
-  constructor
-  . intros o r c id hq
-    rw [<-hiff] at *
-    apply hP.origin_not_leq <;> assumption
-  . intros o r c id x hq hreachable
-    rw [<-hiff] at *
-    apply hP.origin_nearest_reachable <;> assumption
-  . intros x y h_id_eq h_qx h_qy
-    rw [<-hiff] at *
-    apply hP.id_unique x y h_id_eq <;> assumption
-
-theorem push_subset {A} (arr : List (YjsItem A)) (a : YjsItem A) :
-  ∀ x, ArrSet arr x -> ArrSet (a :: arr) x := by
-  intros x hin
-  unfold ArrSet at *
-  simp
-  cases x <;> (simp at *)
-  right; assumption
-
-theorem reachable_in {A} (arr : List (YjsItem A)) (a : YjsPtr A) :
-  IsClosedItemSet (ArrSet arr) ->
-  ∀ x, OriginReachable a x -> ArrSet arr a -> ArrSet arr x := by
-  intros hclosed x hreach hin
-  induction hreach with
-  | reachable_head x a y step h ih =>
-    cases step with
-    | reachable =>
-      simp [ArrSet] at hin
-      apply hclosed.closedLeft at hin
-      apply ih
-      assumption
-    | reachable_right =>
-      simp [ArrSet] at hin
-      apply hclosed.closedRight at hin
-      apply ih
-      assumption
-  | reachable_single _ _ hstep =>
-    cases hstep with
-    | reachable =>
-      simp [ArrSet] at hin
-      apply hclosed.closedLeft at hin
-      assumption
-    | reachable_right =>
-      simp [ArrSet] at hin
-      apply hclosed.closedRight at hin
-      assumption
-
-omit [DecidableEq A] in theorem item_set_invariant_push (arr : List (YjsItem A)) (item : YjsItem A) :
-  ItemSetInvariant (ArrSet arr) ->
-  ArrSetClosed arr ->
-  YjsLt' item.origin item.rightOrigin ->
-  (∀ x, OriginReachable item x -> YjsLeq' x item.origin ∨ YjsLeq' item.rightOrigin x) ->
-  (∀ x : YjsItem A, ArrSet arr x -> x.id = item.id -> x = item) ->
-  ItemSetInvariant (ArrSet (item :: arr)) := by
-  intros hinv hclosed horigin hreach hsameid
-  apply ItemSetInvariant.mk
-  . intros o r c id hitem
-    simp [ArrSet] at hitem
-    cases hitem with
-    | inr hin =>
-      apply hinv.origin_not_leq at hin; assumption
-    | inl heq =>
-      subst heq
-      assumption
-  . intros o r c id x hin hreachable
-    simp [ArrSet] at hin
-    cases hin with
-    | inr hin =>
-      apply hinv.origin_nearest_reachable _ _ _ _ _ hin hreachable
-    | inl heq =>
-      subst heq
-      simp [YjsItem.origin, YjsItem.rightOrigin] at *
-      apply hreach _ hreachable
-  . intros x y h_id_eq h_set_x h_set_y
-    simp [ArrSet] at *
-    cases h_set_x with
-    | inr hinx =>
-      cases h_set_y with
-      | inr hiny =>
-        apply hinv.id_unique _ _ h_id_eq hinx hiny
-      | inl hleq =>
-        subst hleq
-        apply hsameid _ hinx h_id_eq
-    | inl hinx =>
-      subst hinx
-      cases h_set_y with
-      | inr hiny =>
-        obtain h := hsameid y hiny (by rw [h_id_eq])
-        subst h; simp
-      | inl heqy =>
-        subst heqy
-        simp
 
 structure YjsArrInvariant (arr : List (YjsItem A)) : Prop where
   closed : IsClosedItemSet (ArrSet arr)
   item_set_inv : ItemSetInvariant (ArrSet arr)
   sorted : List.Pairwise (fun (x y : YjsItem A) => YjsLt' (A := A) x y) arr
-  unique : List.Pairwise (fun x y => x ≠ y) arr
+  unique : List.Pairwise (fun x y => x.id ≠ y.id) arr
 
 theorem same_yjs_set_unique_aux (xs_all ys_all xs ys : List (YjsItem A)) :
   YjsArrInvariant xs_all ->
@@ -474,23 +183,7 @@ theorem same_yjs_set_unique (xs ys : List (YjsItem A)) :
   . exists []
   . apply hseteq
 
-theorem findPtrIdx_item_exists (arr : Array (YjsItem A)) (x : YjsItem A) :
-  findPtrIdx x arr = Except.ok i ->
-  ∃j, i.toNat? = some j ∧ arr[j]? = some x := by
-  intros hfind
-  simp [findPtrIdx] at hfind
-  generalize heq : Array.findIdx? (fun i => i = x) arr = idx at hfind
-  cases idx <;> cases hfind
-  constructor; constructor
-  . unfold Int.toNat?
-    eq_refl
-  . rw [Array.findIdx?_eq_some_iff_getElem] at heq
-    obtain ⟨ h, h1, h2 ⟩ := heq
-    rw [Array.getElem?_eq_getElem]
-    rw [decide_eq_true_eq] at h1
-    simp; assumption
-
-theorem idx_lt_pairwise {α} {P : α -> α -> Prop} (xs : List α) (i j : Nat) :
+private theorem idx_lt_pairwise {α} {P : α -> α -> Prop} (xs : List α) (i j : Nat) :
   List.Pairwise (fun (x y : α) => P x y) xs ->
   i < j ->
   (hlt_x : i < xs.length) ->
@@ -514,7 +207,7 @@ theorem idx_lt_pairwise {α} {P : α -> α -> Prop} (xs : List α) (i j : Nat) :
         apply hpair
       . omega
 
-omit [DecidableEq A] in theorem getElem_lt_YjsLt' (arr : Array (YjsItem A)) (i j : Nat) :
+omit [DecidableEq A] in private theorem getElem_lt_YjsLt' (arr : Array (YjsItem A)) (i j : Nat) :
   YjsArrInvariant arr.toList ->
   (hij : i < j) ->
   (hjsize : j < arr.size) ->
@@ -645,76 +338,6 @@ theorem findPtrIdx_lt_YjsLt' (arr : Array (YjsItem A)) (x y : YjsPtr A) :
         rw [<-Int.ofNat_lt]
         assumption
 
-theorem findPtrIdx_eq_ok_inj {arr : Array (YjsItem A)} (x y : YjsPtr A) :
-  findPtrIdx x arr = Except.ok i →
-  findPtrIdx y arr = Except.ok i →
-   x = y := by
-  intros heq_x heq_y
-  cases x with
-  | first =>
-    cases y with
-    | first =>
-      simp
-    | last =>
-      simp [findPtrIdx] at heq_x heq_y
-      cases heq_x
-      cases heq_y
-    | itemPtr y =>
-      exfalso
-      simp [findPtrIdx] at heq_x heq_y
-      generalize heq :  Array.findIdx? (fun i => decide (i = y)) arr = idx at *
-      cases idx <;> cases heq_y
-      cases heq_x
-  | last =>
-    cases y with
-    | first =>
-      simp [findPtrIdx] at heq_x heq_y
-      cases heq_x
-      cases heq_y
-    | last =>
-      simp
-    | itemPtr y =>
-      exfalso
-      simp [findPtrIdx] at heq_x heq_y
-      generalize heq :  Array.findIdx? (fun i => decide (i = y)) arr = idx at *
-      cases idx <;> cases heq_y
-      cases heq_x
-      rw [Array.findIdx?_eq_some_iff_findIdx_eq] at heq
-      omega
-  | itemPtr x =>
-    cases y with
-    | first =>
-      exfalso
-      simp [findPtrIdx] at heq_x heq_y
-      generalize heq :  Array.findIdx? (fun i => decide (i = x)) arr = idx at *
-      cases idx <;> cases heq_x
-      cases heq_y
-    | last =>
-      exfalso
-      simp [findPtrIdx] at heq_x heq_y
-      generalize heq :  Array.findIdx? (fun i => decide (i = x)) arr = idx at *
-      cases idx <;> cases heq_x
-      cases heq_y
-      rw [Array.findIdx?_eq_some_iff_findIdx_eq] at heq
-      omega
-    | itemPtr y =>
-      simp [findPtrIdx] at heq_x heq_y
-      generalize heq_x :  Array.findIdx? (fun i => decide (i = x)) arr = idxX at *
-      generalize heq_y :  Array.findIdx? (fun i => decide (i = y)) arr = idxY at *
-      cases idxX <;> cases heq_x
-      cases idxY <;> cases heq_y
-      rw [Array.findIdx?_eq_some_iff_findIdx_eq] at heq_x
-      rw [Array.findIdx?_eq_some_iff_findIdx_eq] at heq_y
-      obtain ⟨ hlt_x, heq_x ⟩ := heq_x
-      obtain ⟨ hlt_y, heq_y ⟩ := heq_y
-      rw [Array.findIdx_eq hlt_x] at heq_x
-      rw [Array.findIdx_eq hlt_y] at heq_y
-      simp at heq_x heq_y
-      obtain ⟨ heq_x, _ ⟩ := heq_x
-      obtain ⟨ heq_y, _ ⟩ := heq_y
-      subst x y
-      simp
-
 theorem findPtrIdx_leq_YjsLeq' (arr : Array (YjsItem A)) (x y : YjsPtr A) :
   YjsArrInvariant arr.toList ->
   findPtrIdx x arr = Except.ok i ->
@@ -841,14 +464,16 @@ theorem YjsLeq'_findPtrIdx_leq (i j : ℤ) (x y : YjsPtr A) (arr : Array (YjsIte
     suffices h : i < j by omega
     apply YjsLt'_findPtrIdx_lt _ _ _ _ _ hinv harrx harry hlt hleft hright
 
-omit [DecidableEq A] in theorem YjsArrayInvariant_lt_neq (arr : Array (YjsItem A)) (i j : Nat) :
+omit [DecidableEq A] in private theorem YjsArrayInvariant_lt_neq (arr : Array (YjsItem A)) (i j : Nat) :
   YjsArrInvariant arr.toList ->
   (hilt : i < arr.size) ->
   (hjlt : j < arr.size) ->
   i < j ->
   arr[i] ≠ arr[j] := by
   intros hinv hilt hjlt hij
-  apply idx_lt_pairwise (P := fun x y => x ≠ y) arr.toList i j hinv.unique hij hilt hjlt
+  have h := idx_lt_pairwise (P := fun x y => x.id ≠ y.id) arr.toList i j hinv.unique hij hilt hjlt
+  simp at h
+  grind only
 
 theorem findPtrIdx_getElem (arr : Array (YjsItem A)) (i :  ℕ) :
   YjsArrInvariant arr.toList ->
@@ -866,58 +491,6 @@ theorem findPtrIdx_getElem (arr : Array (YjsItem A)) (i :  ℕ) :
   . intros j hij heq
     apply YjsArrayInvariant_lt_neq arr j i hinv (by omega) hlt hij (by simp at heq; assumption)
   . assumption
-
-
-theorem findPtrIdx_ge_minus_1 {arr : Array (YjsItem A)} (item : YjsPtr A) :
-  findPtrIdx item arr = Except.ok idx
-  -> idx ≥ -1 := by
-  intros hfind
-  unfold findPtrIdx at hfind
-  cases item with
-  | first =>
-    simp at hfind
-    cases hfind
-    simp
-  | last =>
-    simp at hfind
-    cases hfind
-    omega
-  | itemPtr item =>
-    simp at hfind
-    generalize heq : Array.findIdx? (fun i => decide (i = item)) arr = idx at hfind
-    cases idx with
-    | none =>
-      cases hfind
-    | some idx =>
-      cases hfind
-      omega
-
-theorem findPtrIdx_le_size {arr : Array (YjsItem A)} (item : YjsPtr A) :
-  findPtrIdx item arr = Except.ok idx
-  -> idx ≤ arr.size := by
-  intros hfind
-  unfold findPtrIdx at hfind
-  cases item with
-  | first =>
-    simp at hfind
-    cases hfind
-    omega
-  | last =>
-    simp at hfind
-    cases hfind
-    simp
-  | itemPtr item =>
-    simp at hfind
-    generalize heq : Array.findIdx? (fun i => decide (i = item)) arr = idx at hfind
-    cases idx with
-    | none =>
-      cases hfind
-    | some idx =>
-      cases hfind
-      rw [Array.findIdx?_eq_some_iff_findIdx_eq] at heq
-      obtain ⟨ _, _ ⟩ := heq
-      simp
-      omega
 
 theorem findPtrIdx_origin_leq_newItem_YjsLt' {arr : Array (YjsItem A)} {other newItem : YjsItem A} :
   (∀i, i ∈ arr → i ∈ ls) ->
@@ -940,14 +513,14 @@ theorem findPtrIdx_origin_leq_newItem_YjsLt' {arr : Array (YjsItem A)} {other ne
   intros hsubset hnewItem_in_ls hother_in_ls hclosed harrsetinv harrinv hinv hfindLeft hfindRight hfindOLeft hfindORight h_newItem_origin_lt_other h_origin_lt_newItem_rightOrigin heq_oleft heq_oleft_eq hlt_oleft_newItem
   have hor : YjsLeq' other.rightOrigin newItem ∨ YjsLt' newItem other.rightOrigin := by
     apply yjs_lt_total (P := ArrSet $ ls) <;> try assumption
-    . obtain ⟨ o, r, id, c ⟩ := other
+    . obtain ⟨ o, r, id, c, d ⟩ := other
       apply hclosed.closedRight o r id c
       simp [ArrSet]
       assumption
   cases hor with
   | inl hle =>
     obtain ⟨ _, hle ⟩ := hle
-    obtain ⟨ o, r, id, c ⟩ := other
+    obtain ⟨ o, r, id, c, d ⟩ := other
     constructor
     apply YjsLt.ltRightOrigin
     assumption
@@ -958,18 +531,18 @@ theorem findPtrIdx_origin_leq_newItem_YjsLt' {arr : Array (YjsItem A)} {other ne
     | inl hlt_left =>
       have heq_origin : YjsLt' newItem.origin other.origin := by
         apply findPtrIdx_lt_YjsLt' <;> assumption
-      obtain ⟨ o, r, id, c ⟩ := other
-      obtain ⟨ no, nr, nid, nc ⟩ := newItem
-      simp [YjsItem.origin, YjsItem.rightOrigin] at heq_origin hlt
+      obtain ⟨ o, r, id, c, d ⟩ := other
+      obtain ⟨ no, nr, nid, nc, nd ⟩ := newItem
+      simp at heq_origin hlt
       apply YjsLt'.ltConflict
       apply ConflictLt'.ltOriginDiff <;> try assumption
     | inr heq_origin =>
       subst oLeftIdx
       have heq_origin : newItem.origin = other.origin := by
         apply findPtrIdx_eq_ok_inj _ _ hfindLeft hfindOLeft
-      obtain ⟨ o, r, id, c ⟩ := other
-      obtain ⟨ no, nr, nid, nc ⟩ := newItem
-      simp [YjsItem.origin, YjsItem.rightOrigin, YjsItem.id] at heq_origin heq_oleft_eq hlt
+      obtain ⟨ o, r, id, c, d ⟩ := other
+      obtain ⟨ no, nr, nid, nc, nd ⟩ := newItem
+      simp at heq_origin heq_oleft_eq hlt
       subst no
       apply YjsLt'.ltConflict
       apply ConflictLt'.ltOriginSame <;> try assumption
