LeanYjs/Network/Yjs/YjsNetwork.lean
@@ -1,7 +1,11 @@
 import LeanYjs.Item
-import LeanYjs.Algorithm.Integrate
-import LeanYjs.Algorithm.IntegrateSpec
-import LeanYjs.Algorithm.IntegrateCommutative
+import LeanYjs.Algorithm.Delete.Basic
+import LeanYjs.Algorithm.Delete.Spec
+import LeanYjs.Algorithm.Insert.Basic
+import LeanYjs.Algorithm.Insert.Spec
+import LeanYjs.Algorithm.Commutativity.InsertInsert
+import LeanYjs.Algorithm.Commutativity.InsertDelete
+import LeanYjs.Algorithm.Commutativity.DeleteDelete
 import LeanYjs.Network.CausalNetwork
 import LeanYjs.Network.CausalOrder
 import LeanYjs.Network.OperationNetwork
@@ -11,6 +15,19 @@ section YjsNetwork
 open NetworkModels
 
 abbrev YjsValidItem A := { item : YjsItem A // item.isValid }
+
+def YjsValidItem.id {A} (item : YjsValidItem A) : YjsId :=
+  item.val.id
+
+inductive YjsOperation A where
+| insert (item : YjsValidItem A) : YjsOperation A
+| delete (id deletedId : YjsId) : YjsOperation A
+deriving Repr, DecidableEq
+
+def YjsOperation.id {A} (op : YjsOperation A) : YjsId :=
+  match op with
+  | YjsOperation.insert item => item.val.id
+  | YjsOperation.delete id _ => id
 
 abbrev YjsArray A := { array : Array (YjsItem A) // YjsArrInvariant array.toList }
 
@@ -55,44 +72,61 @@ theorem integrateValid_eq_integrateSafe {A} [DecidableEq A] (item : YjsValidItem
       rfl
     simp
 
-instance : Message (YjsValidItem A) YjsId where
-  messageId item := item.val.id
+def deleteValid {A} [DecidableEq A] (id : YjsId) (state : YjsArray A) : YjsArray A :=
+  let newArr := deleteById state.val id
+  ⟨ newArr, by subst newArr; apply YjsArrInvariant_deleteById; apply state.2 ⟩
 
-instance [DecidableEq A] : Operation (YjsValidItem A) where
+instance : Message (YjsOperation A) YjsId where
+  messageId item := match item with
+  | YjsOperation.insert item => item.val.id
+  | YjsOperation.delete id _ => id
+
+instance [DecidableEq A] : Operation (YjsOperation A) where
   State := { s : Array (YjsItem A) // YjsArrInvariant s.toList }
   Error := IntegrateError
   init := YjsEmptyArray
-  effect item state := integrateValid item state
+  effect item state := match item with
+  | YjsOperation.insert item => integrateValid item state
+  | YjsOperation.delete _id deletedId =>
+    Except.ok <| deleteValid deletedId state
 
-instance [DecidableEq A] : ValidMessage (YjsValidItem A) where
-  isValidMessage state item :=
-    ArrSet state.val.toList item.val.origin
-    ∧ ArrSet state.val.toList item.val.rightOrigin
+def IsValidMessage (state : YjsArray A) (item : YjsOperation A) : Prop :=
+  match item with
+  | YjsOperation.insert item =>
+    ArrSet state.val.toList item.val.origin ∧
+    ArrSet state.val.toList item.val.rightOrigin
+  | YjsOperation.delete _ _ =>
+    True
 
-structure YjsOperationNetwork A [DecidableEq A] extends OperationNetwork (YjsValidItem A) where
-  histories_client_id : forall {e i}, Event.Broadcast e ∈ histories i → e.val.id.clientId = i
-  histories_UniqueId : forall {e i}, histories i = hist1 ++ [Event.Broadcast e] ++ hist2 →
-    interpHistory hist1 Operation.init = Except.ok array → UniqueId e.val (array : YjsArray A).val
+instance [DecidableEq A] : ValidMessage (YjsOperation A) where
+  isValidMessage state item := IsValidMessage state item
 
-theorem foldlM_foldr_effect_comp_eq {A} [DecidableEq A] {network : CausalNetwork (YjsValidItem A)} (items : List (CausalNetworkElem (YjsValidItem A) network)) (init : YjsArray A) :
-  List.foldlM (fun acc item => integrateValid item acc) init (List.map (fun item => item.elem) items) =
+def YjsOperation.UniqueId {A} (op : YjsOperation A) (state : YjsArray A) : Prop :=
+    ∀x ∈ state.val, x.id.clientId = op.id.clientId → x.id.clock < op.id.clock
+
+structure YjsOperationNetwork A [DecidableEq A] extends OperationNetwork (YjsOperation A) where
+  histories_client_id : forall {e i}, Event.Broadcast e ∈ histories i → e.id.clientId = i
+  histories_UniqueId : forall {e i} {array : YjsArray A}, histories i = hist1 ++ [Event.Broadcast e] ++ hist2 →
+    interpHistory hist1 Operation.init = Except.ok array → YjsOperation.UniqueId e array
+
+theorem foldlM_foldr_effect_comp_eq {A} [DecidableEq A] {network : CausalNetwork (YjsOperation A)} (items : List (CausalNetworkElem (YjsOperation A) network)) (init : YjsArray A) :
+  List.foldlM (fun acc item => Operation.effect item acc) init (List.map (fun item => item.elem) items) =
   List.foldr effect_comp (fun s => Except.ok s) (items.map (fun a => Operation.effect a)) init := by
   induction items generalizing init with
   | nil =>
     simp
     eq_refl
   | cons item items ih =>
-    simp [effect_comp, bind, Except.bind, Operation.effect]
-    generalize h_init' : integrateValid item.elem init = init' at *
+    simp [effect_comp, bind, Except.bind]
+    generalize h_init' : Operation.effect item.elem init = init' at *
     cases init' with
     | error err =>
       simp
     | ok state' =>
       simp
       rw [ih]
-      eq_refl
 
-theorem interpDeliveredMessages_foldr_effect_comp_eq : forall {A} [DecidableEq A] {network : CausalNetwork (YjsValidItem A)} (items : List (CausalNetworkElem (YjsValidItem A) network)),
+theorem interpDeliveredMessages_foldr_effect_comp_eq : forall {A} [DecidableEq A] {network : CausalNetwork (YjsOperation A)} (items : List (CausalNetworkElem (YjsOperation A) network)),
   interpDeliveredOps items Operation.init =
   List.foldr effect_comp (fun s => Except.ok s) (items.map (fun a => Operation.effect a)) YjsEmptyArray := by
   intros A _ network items
@@ -141,7 +175,7 @@ theorem Except.map_eq_eq {α β ε : Type} (f : α → β) {e1 e2 : Except ε α
       have h_val_eq : val1 = val2 := h_f val1 val2 h_eq
       rw [h_val_eq]
 
-theorem same_history_not_hb_concurrent {A} [DecidableEq A] {network : CausalNetwork (YjsValidItem A)} {i : ClientId} {a b : YjsValidItem A} :
+theorem same_history_not_hb_concurrent {A} [DecidableEq A] {network : CausalNetwork (YjsOperation A)} {i : ClientId} {a b : YjsOperation A} :
   Event.Broadcast a ∈ network.histories i →
   Event.Broadcast b ∈ network.histories i →
   ¬hb_concurrent inferInstance (CausalNetworkElem.mk (network := network) a) (CausalNetworkElem.mk (network := network) b) := by
@@ -192,8 +226,8 @@ theorem same_history_not_hb_concurrent {A} [DecidableEq A] {network : CausalNetw
       grind
 
 theorem integrateValid_exists_insertIdxIfBounds {A : Type} [inst : DecidableEq A]
-  {init : Operation.State (YjsValidItem A)} {item : YjsValidItem A}
-  {state' : Operation.State (YjsValidItem A)} :
+  {init : YjsArray A} {item : YjsValidItem A}
+  {state' : YjsArray A} :
   (h_effect : integrateValid item init = Except.ok state') →
   ∃ i, state'.val = init.val.insertIdxIfInBounds i ↑item := by
   intro h_effect
@@ -222,17 +256,18 @@ theorem integrateValid_exists_insertIdxIfBounds {A : Type} [inst : DecidableEq A
   have ⟨ i, _, h_eq, _ ⟩ := YjsArrInvariant_integrateSafe item.val init.val state'.val init.prop item.prop h_eq
   use i
 
-theorem interpOps_ArrSet {A} [DecidableEq A] {items : List (Event (YjsValidItem A))} {state init : Operation.State (YjsValidItem A)} {x : YjsItem A}:
+theorem interpOps_ArrSet {A} [DecidableEq A] {items : List (Event (YjsOperation A))} {state init : Operation.State (YjsOperation A)} {x : YjsItem A}:
   interpHistory items init = Except.ok state →
   ArrSet state.val.toList x →
-  ArrSet init.val.toList x ∨ ∃y, y.val = x ∧ Event.Deliver y ∈ items  := by
+  (∃y, ArrSet init.val.toList (YjsPtr.itemPtr y) ∧ y.id = x.id) ∨
+  (∃y, y.val.id = x.id ∧ Event.Deliver (YjsOperation.insert y) ∈ items) := by
   intros h_interp h_in_state
   induction items generalizing init state x with
   | nil =>
     simp [interpHistory, interpOps, pure] at h_interp
     cases h_interp
     simp [ArrSet] at h_in_state |-
-    assumption
+    use x
   | cons e items ih =>
     simp [interpHistory, interpOps] at h_interp
     cases e with
@@ -248,46 +283,69 @@ theorem interpOps_ArrSet {A} [DecidableEq A] {items : List (Event (YjsValidItem 
         use y
         constructor; assumption
         simp; assumption
-    | Deliver item =>
-      simp at h_interp
-      generalize h_effect : Operation.effect item init = state' at *
-      cases state' with
-      | error err =>
-        cases h_interp
-      | ok state' =>
-        rw [ok_bind] at h_interp
-        apply ih h_interp at h_in_state
+    | Deliver op =>
+      cases op with
+      | delete _ deletedId =>
+        simp [Operation.effect] at h_interp
+        apply ih (x := x) h_interp at h_in_state
         cases h_in_state with
-        | inl h_init_mem =>
-          simp [Operation.effect] at h_effect
-          have ⟨ _, h_insert ⟩ : ∃i, state'.val = init.val.insertIdxIfInBounds i item := by
-            apply integrateValid_exists_insertIdxIfBounds h_effect
-          rw [h_insert] at h_init_mem
-          simp [Array.insertIdxIfInBounds] at h_init_mem
-          split at h_init_mem
-          . simp [ArrSet] at h_init_mem
-            rw [List.mem_insertIdx (by assumption)] at h_init_mem
-            cases h_init_mem with
-            | inl h_mem =>
-              right; subst x; simp
-              obtain ⟨ _, _ ⟩ := item
-              simp; assumption
-            | inr h_eq =>
-              left; assumption
-          . left; assumption
-        | inr h_in_state =>
-          obtain ⟨ y, h_y_val, h_y_mem ⟩ := h_in_state
+        | inl h =>
+          obtain ⟨ y, h_mem, h_y_id ⟩ := h
+          simp [ArrSet, deleteValid, deleteById] at h_mem
+          obtain ⟨ a, h_a_mem, h_a_eq ⟩ := h_mem
+          left; use a; constructor; simp [ArrSet]; assumption
+          rw [<-h_y_id, <-h_a_eq, deleteItemById_id]
+        | inr h =>
+          obtain ⟨ y, h_y_val, h_y_mem ⟩ := h
           right; use y
           simp; constructor; assumption
-          right; assumption
+          assumption
+      | insert item =>
+        simp at h_interp
+        generalize h_effect : Operation.effect (YjsOperation.insert item) init = state' at *
+        cases state' with
+        | error err =>
+          cases h_interp
+        | ok state' =>
+          rw [ok_bind] at h_interp
+          apply ih h_interp at h_in_state
+          cases h_in_state with
+          | inl h_init_mem =>
+            simp [Operation.effect] at h_effect
+            have ⟨ _, h_insert ⟩ : ∃i, state'.val = init.val.insertIdxIfInBounds i item := by
+              apply integrateValid_exists_insertIdxIfBounds h_effect
+            rw [h_insert] at h_init_mem
+            simp [Array.insertIdxIfInBounds] at h_init_mem
+            split at h_init_mem
+            . simp [ArrSet] at h_init_mem
+              obtain ⟨ y, h_y_mem, h_y_id ⟩ := h_init_mem
+              rw [List.mem_insertIdx (by assumption)] at h_y_mem
+              cases h_y_mem with
+              | inl h_mem =>
+                right
+                use item
+                constructor
+                grind only
+                simp
+              | inr h_eq =>
+                left; use y; constructor; simp [ArrSet] at *; assumption
+                assumption
+            . left; assumption
+          | inr h_in_state =>
+            obtain ⟨ y, h_y_val, h_y_mem ⟩ := h_in_state
+            right; use y
+            simp; constructor; assumption
+            right; assumption
 
-theorem OriginReachable_HappensBefore {A : Type} [inst : DecidableEq A]
-  {network : YjsOperationNetwork A} {i : ClientId} {a b : CausalNetworkElem (YjsValidItem A) network.toCausalNetwork} :
+theorem OriginReachable_HappensBefore {A : Type} [DecidableEq A]
+  {network : YjsOperationNetwork A} {i : ClientId} {a b : CausalNetworkElem (YjsOperation A) network.toCausalNetwork} {item_a item_b : YjsValidItem A} :
   a ∈ network.toDeliverMessages i →
   b ∈ network.toDeliverMessages i →
-  OriginReachable (YjsPtr.itemPtr a.elem.val) (YjsPtr.itemPtr b.elem.val) →
+  a.elem = YjsOperation.insert item_a →
+  b.elem = YjsOperation.insert item_b →
+  OriginReachable (YjsPtr.itemPtr item_a.val) (YjsPtr.itemPtr item_b.val) →
   b ≤ a := by
-  intros h_a_mem h_b_mem h_reachable
+  intros h_a_mem h_b_mem h_item_a h_item_b h_reachable
 
   simp [CausalNetwork.toDeliverMessages] at h_b_mem h_a_mem
   replace ⟨ a, h_a_mem, h_a_eq ⟩ := h_a_mem
@@ -325,10 +383,12 @@ theorem OriginReachable_HappensBefore {A : Type} [inst : DecidableEq A]
   simp at h_a_eq h_b_eq
   subst h_a_eq h_b_eq
 
+  simp at h_item_a h_item_b
+  subst a' b'
   simp [ValidMessage.isValidMessage] at h_valid_message_a
   obtain ⟨ h_a_origin_in_state_a, h_a_rightOrigin_in_state_a ⟩ := h_valid_message_a
 
-  generalize h_a_ptr_def : YjsPtr.itemPtr a'.val = a_ptr at *
+  generalize h_a_ptr_def : YjsPtr.itemPtr item_a.val = a_ptr at *
 
   have h_OriginReachableStep_ArrSet : ∀ x,
     OriginReachableStep a_ptr x → ArrSet state_a.val.toList x := by
@@ -337,15 +397,15 @@ theorem OriginReachable_HappensBefore {A : Type} [inst : DecidableEq A]
     | reachable o r id c =>
       simp at h_a_ptr_def
       rw [h_a_ptr_def] at h_a_origin_in_state_a
-      simp [YjsItem.origin] at h_a_origin_in_state_a
+      simp at h_a_origin_in_state_a
       assumption
     | reachable_right o r id c =>
       simp at h_a_ptr_def
       rw [h_a_ptr_def] at h_a_rightOrigin_in_state_a
-      simp [YjsItem.rightOrigin] at h_a_rightOrigin_in_state_a
+      simp at h_a_rightOrigin_in_state_a
       assumption
 
-  have h_b_in_state_a : ArrSet (state_a.val.toList) b'.val := by
+  have h_b_in_state_a : ArrSet (state_a.val.toList) item_b.val := by
     cases h_reachable with
     | reachable_single _ _ h_step =>
       apply h_OriginReachableStep_ArrSet _ h_step
@@ -357,86 +417,147 @@ theorem OriginReachable_HappensBefore {A : Type} [inst : DecidableEq A]
       apply reachable_in _ _ h_closed _ h_reach_tail h_step
 
   apply interpOps_ArrSet h_state_a at h_b_in_state_a
-  simp [ArrSet, Operation.init, YjsEmptyArray] at h_b_in_state_a
-  obtain ⟨ h_b_in_items_mem, h_b_in_items_eq ⟩ := h_b_in_state_a
+  cases h_b_in_state_a with
+  | inl h_b_in_init =>
+    simp [ArrSet, Operation.init, YjsEmptyArray] at h_b_in_init
+  | inr h_b_in_items =>
+    obtain ⟨ item_b', h_b_id_eq,  h_b_in_items_eq ⟩ := h_b_in_items
 
-  rw [List.mem_iff_append] at h_b_in_items_eq
-  obtain ⟨ pre_b'', post_b'', h_b_in_items_history ⟩ := h_b_in_items_eq
+    rw [List.mem_iff_append] at h_b_in_items_eq
+    obtain ⟨ pre_b'', post_b'', h_b_in_items_history ⟩ := h_b_in_items_eq
 
-  right
-  apply HappensBefore.broadcast_deliver_local (i := j_a)
+    right
+    apply HappensBefore.broadcast_deliver_local (i := j_a)
 
-  use pre_b'', post_b'', post_a
+    use pre_b'', post_b'', post_a
 
-  rw [h_a_history, h_b_in_items_history]
+    rw [h_a_history, h_b_in_items_history]
+    simp at *
+    have h_b_id_eq : Message.messageId (YjsOperation.insert item_b') = Message.messageId (YjsOperation.insert item_b) := by
+      assumption
+    have h_item_b'_in_ja : Event.Deliver (YjsOperation.insert item_b') ∈ network.histories j_a := by
+      rw [h_a_history, h_b_in_items_history]; simp
+    apply network.deliver_has_a_cause at h_item_b'_in_ja
+    obtain ⟨ j_b', h_item_b'_in_ja_history ⟩ := h_item_b'_in_ja
+    apply network.msg_id_unique (i := j_b') (j := j_b) at h_b_id_eq
+    . obtain ⟨ _, h_eq ⟩ := h_b_id_eq
+      simp at h_eq
+      subst item_b'
+      rfl
+    . assumption
+    . rw [h_b_history]; simp
+
+theorem hb_concurrent_diff_id {A : Type} [inst : DecidableEq A]
+  (network : YjsOperationNetwork A) (i : ClientId)
+  (a : CausalNetworkElem (YjsOperation A) network.toCausalNetwork)
+  (h_a_mem : a ∈ network.toDeliverMessages i)
+  (b : CausalNetworkElem (YjsOperation A) network.toCausalNetwork)
+  (h_b_mem : b ∈ network.toDeliverMessages i)
+  (h_a_b_happens_before : hb_concurrent inferInstance a b) :
+  a.elem.id.clientId ≠ b.elem.id.clientId := by
+  intros h_eq
+  simp [CausalNetwork.toDeliverMessages] at h_a_mem h_b_mem
+  obtain ⟨ a', h_a'_mem, h_a'_pos ⟩ := h_a_mem
+  obtain ⟨ b', h_b'_mem, h_b'_pos ⟩ := h_b_mem
+
+  have ⟨ a', h_a ⟩ : ∃ a'', Event.Deliver a'' = a' := by
+    cases a' with
+    | Deliver it =>
+      use it
+    | Broadcast e =>
+      simp at h_a'_pos
+
+  have ⟨ b', h_b ⟩ : ∃ b'', Event.Deliver b'' = b' := by
+    cases b' with
+    | Deliver it =>
+      use it
+    | Broadcast e =>
+      simp at h_b'_pos
+
+  subst h_a h_b
+
+  apply network.deliver_has_a_cause at h_a'_mem
+  obtain ⟨ i_a, h_a'_mem_hist ⟩ := h_a'_mem
+  apply network.deliver_has_a_cause at h_b'_mem
+  obtain ⟨ i_b, h_b'_mem_hist ⟩ := h_b'_mem
+
+  have h_i_a_eq_i_b : i_a = i_b := by
+    apply network.histories_client_id at h_a'_mem_hist
+    apply network.histories_client_id at h_b'_mem_hist
+    simp at *
+    subst a b
+    subst i_a i_b
+    assumption
+
+  subst i_a
   simp at *
+  subst a b
+  apply same_history_not_hb_concurrent h_a'_mem_hist h_b'_mem_hist h_a_b_happens_before
 
 theorem YjsOperationNetwork_concurrentCommutative {A} [DecidableEq A] (network : YjsOperationNetwork A) (i : ClientId) :
   concurrent_commutative inferInstance (network.toCausalNetwork.toDeliverMessages i) := by
   intros a b h_a_mem h_b_mem h_a_b_happens_before
   funext s
   simp [Operation.State, Operation.Error] at *
-  simp [effect_comp, effect, Operation.effect]
+  simp [effect_comp, effect]
   apply Except.map_eq_eq (f := fun (x : YjsArray A) => x.val)
   . intros x y h_eq
     apply Subtype_eq_of_val
     exact h_eq
-  . rw [integrateValid_bind_integrateSafe]
-    rw [integrateValid_bind_integrateSafe]
-    apply integrate_commutative
-    . obtain ⟨ s, h_s ⟩ := s
-      simp; assumption
-    . intros h_eq
-      simp [CausalNetwork.toDeliverMessages] at h_a_mem h_b_mem
-      obtain ⟨ a', h_a'_mem, h_a'_pos ⟩ := h_a_mem
-      obtain ⟨ b', h_b'_mem, h_b'_pos ⟩ := h_b_mem
-
-      have ⟨ a', h_a ⟩ : ∃ a'', Event.Deliver a'' = a' := by
-        cases a' with
-        | Deliver it =>
-          use it
-        | Broadcast e =>
-          simp at h_a'_pos
-
-      have ⟨ b', h_b ⟩ : ∃ b'', Event.Deliver b'' = b' := by
-        cases b' with
-        | Deliver it =>
-          use it
-        | Broadcast e =>
-          simp at h_b'_pos
-
-      subst h_a h_b
-
-      apply network.deliver_has_a_cause at h_a'_mem
-      obtain ⟨ i_a, h_a'_mem_hist ⟩ := h_a'_mem
-      apply network.deliver_has_a_cause at h_b'_mem
-      obtain ⟨ i_b, h_b'_mem_hist ⟩ := h_b'_mem
-
-      have h_i_a_eq_i_b : i_a = i_b := by
-        apply network.histories_client_id at h_a'_mem_hist
-        apply network.histories_client_id at h_b'_mem_hist
-        simp at *
-        subst a b
-        simp at *
-        subst i_a i_b
-        assumption
-
-      subst i_a
-      simp at *
-      subst a b
-      apply same_history_not_hb_concurrent h_a'_mem_hist h_b'_mem_hist h_a_b_happens_before
-    . intros h_reachable
-      obtain ⟨ _, h_b_hb_a ⟩ := h_a_b_happens_before
-      apply h_b_hb_a
-      apply OriginReachable_HappensBefore h_a_mem h_b_mem h_reachable
-    . intros h_reachable
-      obtain ⟨ h_a_hb_b, _ ⟩ := h_a_b_happens_before
-      apply h_a_hb_b
-      apply OriginReachable_HappensBefore h_b_mem h_a_mem h_reachable
-    . obtain ⟨ a, _ ⟩ := a
-      assumption
-    . obtain ⟨ b, _ ⟩ := b
-      assumption
+  . obtain ⟨ a ⟩ := a
+    obtain ⟨ b ⟩ := b
+    cases a with
+    | insert a =>
+      cases b with
+      | insert b =>
+        conv =>
+          lhs
+          enter [2]
+          simp [Operation.effect]
+        rw [integrateValid_bind_integrateSafe]
+        conv =>
+          rhs
+          enter [2]
+          simp [Operation.effect]
+        rw [integrateValid_bind_integrateSafe]
+        apply integrate_commutative
+        . obtain ⟨ s, h_s ⟩ := s
+          simp; assumption
+        . apply hb_concurrent_diff_id _ _
+            (a := ⟨ YjsOperation.insert a ⟩) (b := ⟨YjsOperation.insert b ⟩) h_a_mem h_b_mem h_a_b_happens_before
+        . intros h_reachable
+          obtain ⟨ _, h_b_hb_a ⟩ := h_a_b_happens_before
+          apply h_b_hb_a
+          apply OriginReachable_HappensBefore h_a_mem h_b_mem rfl rfl h_reachable
+        . intros h_reachable
+          obtain ⟨ h_a_hb_b, _ ⟩ := h_a_b_happens_before
+          apply h_a_hb_b
+          apply OriginReachable_HappensBefore h_b_mem h_a_mem rfl rfl h_reachable
+        . obtain ⟨ a, _ ⟩ := a
+          assumption
+        . obtain ⟨ b, _ ⟩ := b
+          assumption
+      | delete _ deletedId =>
+        simp [Operation.State, Operation.Error, Operation.effect]
+        simp [deleteValid]
+        rw [<-bind_map_left (f := fun (x : YjsArray A) => x.val) (g := fun arr => Except.ok (deleteById arr deletedId)),
+            integrateValid_eq_integrateSafe,
+            integrateSafe_deleteById_commutative]
+        simp [bind, Except.bind]
+        rw [integrateValid_eq_integrateSafe]
+    | delete _ deletedId =>
+      cases b with
+      | insert b =>
+        simp [Operation.State, Operation.Error, Operation.effect]
+        simp [deleteValid]
+        rw [<-bind_map_left (f := fun (x : YjsArray A) => x.val) (g := fun arr => Except.ok (deleteById arr deletedId)),
+            integrateValid_eq_integrateSafe,
+            integrateSafe_deleteById_commutative]
+        simp [bind, Except.bind]
+        rw [integrateValid_eq_integrateSafe]
+      | delete _ deletedId' =>
+        simp [Operation.Error, Operation.effect, deleteValid, bind, Except.bind]
+        apply deleteById_commutative
 
 theorem YjsOperationNetwork_converge' : forall {A} [DecidableEq A] (network : YjsOperationNetwork A) (i j : ClientId) (res₀ res₁ : YjsArray A),
   let hist_i := network.toDeliverMessages i
@@ -450,7 +571,7 @@ theorem YjsOperationNetwork_converge' : forall {A} [DecidableEq A] (network : Yj
 
   subst hist_i hist_j
 
-  let hb : CausalOrder (CausalNetworkElem (YjsValidItem A) network.toCausalNetwork) := inferInstance
+  let hb : CausalOrder (CausalNetworkElem (YjsOperation A) network.toCausalNetwork) := inferInstance
   have h_consistent_i : hb_consistent hb (network.toCausalNetwork.toDeliverMessages i) := by
     apply hb_consistent_local_history
   have h_consistent_j : hb_consistent hb (network.toCausalNetwork.toDeliverMessages j) := by
