LeanYjs/Order/ItemOrder.lean
@@ -14,8 +14,8 @@ inductive OriginLt {A} : YjsPtr A -> YjsPtr A -> Prop where
   | lt_first_last : OriginLt YjsPtr.first YjsPtr.last
 
 inductive OriginReachableStep {A} : YjsPtr A -> YjsPtr A -> Prop where
-  | reachable : forall o r id c, OriginReachableStep (YjsItem.item o r id c) o
-  | reachable_right : forall o r id c, OriginReachableStep (YjsItem.item o r id c) r
+  | reachable : forall o r id c d, OriginReachableStep (YjsItem.mk o r id c d) o
+  | reachable_right : forall o r id c d, OriginReachableStep (YjsItem.mk o r id c d) r
 
 inductive OriginReachable {A} : YjsPtr A -> YjsPtr A -> Prop where
   | reachable_single : forall x y, OriginReachableStep x y -> OriginReachable x y
@@ -25,25 +25,25 @@ mutual
   inductive YjsLt {A : Type} : Nat -> YjsPtr A -> YjsPtr A -> Prop where
     | ltConflict h i1 i2 : ConflictLt h i1 i2 -> YjsLt (h + 1) i1 i2
     | ltOriginOrder i1 i2 : OriginLt i1 i2 -> YjsLt 0 i1 i2
-    | ltOrigin h x o r id c : YjsLeq h x o -> YjsLt (h + 1) x (YjsItem.item o r id c)
-    | ltRightOrigin h o r id c x : YjsLeq h r x -> YjsLt (h + 1) (YjsItem.item o r id c) x
+    | ltOrigin h x o r id c d : YjsLeq h x o -> YjsLt (h + 1) x (YjsItem.mk o r id c d)
+    | ltRightOrigin h o r id c d x : YjsLeq h r x -> YjsLt (h + 1) (YjsItem.mk o r id c d) x
 
   inductive YjsLeq {A : Type} : Nat -> YjsPtr A -> YjsPtr A -> Prop where
     | leqSame x : YjsLeq h x x
     | leqLt h x y : YjsLt h x y -> YjsLeq (h + 1) x y
 
   inductive ConflictLt {A : Type} : Nat -> YjsPtr A -> YjsPtr A -> Prop where
-    | ltOriginDiff h1 h2 h3 h4 l1 l2 r1 r2 id1 id2 c1 c2 :
+    | ltOriginDiff h1 h2 h3 h4 l1 l2 r1 r2 id1 id2 c1 c2 d1 d2 :
       YjsLt h1 l2 l1
-      -> YjsLt h2 (YjsItem.item l1 r1 id1 c1) r2
-      -> YjsLt h3 l1 (YjsItem.item l2 r2 id2 c2)
-      -> YjsLt h4 (YjsItem.item l2 r2 id2 c2) r1
-      -> ConflictLt (max4 h1 h2 h3 h4 + 1) (YjsItem.item l1 r1 id1 c1) (YjsItem.item l2 r2 id2 c2)
-    | ltOriginSame h1 h2 l r1 r2 id1 id2 (c1 c2 : A) :
-      YjsLt h1 (YjsItem.item l r1 id1 c1) r2
-      -> YjsLt h2 (YjsItem.item l r2 id2 c2) r1
+      -> YjsLt h2 (YjsItem.mk l1 r1 id1 c1 d1) r2
+      -> YjsLt h3 l1 (YjsItem.mk l2 r2 id2 c2 d2)
+      -> YjsLt h4 (YjsItem.mk l2 r2 id2 c2 d2) r1
+      -> ConflictLt (max4 h1 h2 h3 h4 + 1) (YjsItem.mk l1 r1 id1 c1 d1) (YjsItem.mk l2 r2 id2 c2 d2)
+    | ltOriginSame h1 h2 l r1 r2 id1 id2 (c1 c2 : A) (d1 d2 : Bool) :
+      YjsLt h1 (YjsItem.mk l r1 id1 c1 d1) r2
+      -> YjsLt h2 (YjsItem.mk l r2 id2 c2 d2) r1
       -> id1 < id2
-      -> ConflictLt (max h1 h2 + 1) (YjsItem.item l r1 id1 c1) (YjsItem.item l r2 id2 c2)
+      -> ConflictLt (max h1 h2 + 1) (YjsItem.mk l r1 id1 c1 d1) (YjsItem.mk l r2 id2 c2 d2)
 end
 
 def ConflictLt' {A} (i1 i2 : YjsPtr A) : Prop :=
@@ -57,10 +57,10 @@ def YjsLeq' {A} (x y : YjsPtr A) : Prop :=
 
 theorem ConflictLt'.ltOriginDiff {A : Type} (l1 l2 r1 r2 : YjsPtr A) (id1 id2 : YjsId) (c1 c2 : A) :
   YjsLt' l2 l1
-  -> YjsLt' (YjsItem.item l1 r1 id1 c1) r2
-  -> YjsLt' l1 (YjsItem.item l2 r2 id2 c2)
-  -> YjsLt' (YjsItem.item l2 r2 id2 c2) r1
-  -> ConflictLt' (A := A) (YjsItem.item l1 r1 id1 c1) (YjsItem.item l2 r2 id2 c2) := by
+  -> YjsLt' (YjsItem.mk l1 r1 id1 c1 d1) r2
+  -> YjsLt' l1 (YjsItem.mk l2 r2 id2 c2 d2)
+  -> YjsLt' (YjsItem.mk l2 r2 id2 c2 d2) r1
+  -> ConflictLt' (A := A) (YjsItem.mk l1 r1 id1 c1 d1) (YjsItem.mk l2 r2 id2 c2 d2) := by
   intros hlt1 hlt2 hlt3 hlt4
   obtain ⟨ h1, hlt1 ⟩ := hlt1
   obtain ⟨ h2, hlt2 ⟩ := hlt2
@@ -69,11 +69,11 @@ theorem ConflictLt'.ltOriginDiff {A : Type} (l1 l2 r1 r2 : YjsPtr A) (id1 id2 : 
   constructor
   apply ConflictLt.ltOriginDiff <;> try assumption
 
-theorem ConflictLt'.ltOriginSame {A : Type} (l r1 r2 : YjsPtr A) (id1 id2 : YjsId) (c1 c2 : A) :
-  YjsLt' (YjsItem.item l r1 id1 c1) r2
-  -> YjsLt' (YjsItem.item l r2 id2 c2) r1
+theorem ConflictLt'.ltOriginSame {A : Type} (l r1 r2 : YjsPtr A) (id1 id2 : YjsId) (c1 c2 : A) (d1 d2 : Bool) :
+  YjsLt' (YjsItem.mk l r1 id1 c1 d1) r2
+  -> YjsLt' (YjsItem.mk l r2 id2 c2 d2) r1
   -> id1 < id2
-  -> ConflictLt' (A := A) (YjsItem.item l r1 id1 c1) (YjsItem.item l r2 id2 c2) := by
+  -> ConflictLt' (A := A) (YjsItem.mk l r1 id1 c1 d1) (YjsItem.mk l r2 id2 c2 d2) := by
   intros hlt1 hlt2 hlt3
   obtain ⟨ h1, hlt1 ⟩ := hlt1
   obtain ⟨ h2, hlt2 ⟩ := hlt2
@@ -92,13 +92,13 @@ theorem YjsLt'.ltOriginOrder {A : Type} (i1 i2 : YjsPtr A) : OriginLt i1 i2 -> Y
   constructor
   apply YjsLt.ltOriginOrder; assumption
 
-theorem YjsLt'.ltOrigin {A : Type} (x o r : YjsPtr A) id c : YjsLeq' x o -> YjsLt' x (YjsItem.item o r id c) := by
+theorem YjsLt'.ltOrigin {A : Type} (x o r : YjsPtr A) id c d : YjsLeq' x o -> YjsLt' x (YjsItem.mk o r id c d) := by
   intros hleq
   obtain ⟨ h, hleq ⟩ := hleq
   constructor
   apply YjsLt.ltOrigin <;> try assumption
 
-theorem YjsLt'.ltRightOrigin {A : Type} (o r : YjsPtr A) id c x : YjsLeq' r x -> YjsLt' (YjsItem.item o r id c) x := by
+theorem YjsLt'.ltRightOrigin {A : Type} (o r : YjsPtr A) id c d x : YjsLeq' r x -> YjsLt' (YjsItem.mk o r id c d) x := by
   intros hleq
   obtain ⟨ h, hleq ⟩ := hleq
   constructor
@@ -143,10 +143,10 @@ theorem yjs_lt_cases A h (x y : YjsPtr A) :
       left; simp
     | lt_last =>
       right; left; simp
-  | ltOrigin h x o r id c hlt =>
+  | ltOrigin h x o r id c d hlt =>
     right; right; right; left; simp
     constructor; assumption
-  | ltRightOrigin h o r id c x hlt =>
+  | ltRightOrigin h o r id c d x hlt =>
     right; right; left; simp
     constructor; assumption
 
