LeanYjs/Algorithm/Basic.lean
@@ -1,0 +1,2 @@
+inductive IntegrateError where
+| error : IntegrateError
