LeanYjs/Algorithm/Insert/Lemmas.lean
@@ -1,0 +1,140 @@
+import LeanYjs.Algorithm.Insert.Basic
+
+variable {A : Type} [DecidableEq A]
+
+theorem findPtrIdx_item_exists (arr : Array (YjsItem A)) (x : YjsItem A) :
+  findPtrIdx x arr = Except.ok i ->
+  ∃j, i.toNat? = some j ∧ arr[j]? = some x := by
+  intros hfind
+  simp [findPtrIdx] at hfind
+  generalize heq : Array.findIdx? (fun i => i = x) arr = idx at hfind
+  cases idx <;> cases hfind
+  constructor; constructor
+  . unfold Int.toNat?
+    eq_refl
+  . rw [Array.findIdx?_eq_some_iff_getElem] at heq
+    obtain ⟨ h, h1, h2 ⟩ := heq
+    rw [Array.getElem?_eq_getElem]
+    rw [decide_eq_true_eq] at h1
+    simp; assumption
+
+theorem findPtrIdx_eq_ok_inj {arr : Array (YjsItem A)} (x y : YjsPtr A) :
+  findPtrIdx x arr = Except.ok i →
+  findPtrIdx y arr = Except.ok i →
+   x = y := by
+  intros heq_x heq_y
+  cases x with
+  | first =>
+    cases y with
+    | first =>
+      simp
+    | last =>
+      simp [findPtrIdx] at heq_x heq_y
+      cases heq_x
+      cases heq_y
+    | itemPtr y =>
+      exfalso
+      simp [findPtrIdx] at heq_x heq_y
+      generalize heq :  Array.findIdx? (fun i => decide (i = y)) arr = idx at *
+      cases idx <;> cases heq_y
+      cases heq_x
+  | last =>
+    cases y with
+    | first =>
+      simp [findPtrIdx] at heq_x heq_y
+      cases heq_x
+      cases heq_y
+    | last =>
+      simp
+    | itemPtr y =>
+      exfalso
+      simp [findPtrIdx] at heq_x heq_y
+      generalize heq :  Array.findIdx? (fun i => decide (i = y)) arr = idx at *
+      cases idx <;> cases heq_y
+      cases heq_x
+      rw [Array.findIdx?_eq_some_iff_findIdx_eq] at heq
+      omega
+  | itemPtr x =>
+    cases y with
+    | first =>
+      exfalso
+      simp [findPtrIdx] at heq_x heq_y
+      generalize heq :  Array.findIdx? (fun i => decide (i = x)) arr = idx at *
+      cases idx <;> cases heq_x
+      cases heq_y
+    | last =>
+      exfalso
+      simp [findPtrIdx] at heq_x heq_y
+      generalize heq :  Array.findIdx? (fun i => decide (i = x)) arr = idx at *
+      cases idx <;> cases heq_x
+      cases heq_y
+      rw [Array.findIdx?_eq_some_iff_findIdx_eq] at heq
+      omega
+    | itemPtr y =>
+      simp [findPtrIdx] at heq_x heq_y
+      generalize heq_x :  Array.findIdx? (fun i => decide (i = x)) arr = idxX at *
+      generalize heq_y :  Array.findIdx? (fun i => decide (i = y)) arr = idxY at *
+      cases idxX <;> cases heq_x
+      cases idxY <;> cases heq_y
+      rw [Array.findIdx?_eq_some_iff_findIdx_eq] at heq_x
+      rw [Array.findIdx?_eq_some_iff_findIdx_eq] at heq_y
+      obtain ⟨ hlt_x, heq_x ⟩ := heq_x
+      obtain ⟨ hlt_y, heq_y ⟩ := heq_y
+      rw [Array.findIdx_eq hlt_x] at heq_x
+      rw [Array.findIdx_eq hlt_y] at heq_y
+      simp at heq_x heq_y
+      obtain ⟨ heq_x, _ ⟩ := heq_x
+      obtain ⟨ heq_y, _ ⟩ := heq_y
+      subst x y
+      simp
+
+theorem findPtrIdx_ge_minus_1 {arr : Array (YjsItem A)} (item : YjsPtr A) :
+  findPtrIdx item arr = Except.ok idx
+  -> idx ≥ -1 := by
+  intros hfind
+  unfold findPtrIdx at hfind
+  cases item with
+  | first =>
+    simp at hfind
+    cases hfind
+    simp
+  | last =>
+    simp at hfind
+    cases hfind
+    omega
+  | itemPtr item =>
+    simp at hfind
+    generalize heq : Array.findIdx? (fun i => decide (i = item)) arr = idx at hfind
+    cases idx with
+    | none =>
+      cases hfind
+    | some idx =>
+      cases hfind
+      omega
+
+theorem findPtrIdx_le_size {arr : Array (YjsItem A)} (item : YjsPtr A) :
+  findPtrIdx item arr = Except.ok idx
+  -> idx ≤ arr.size := by
+  intros hfind
+  unfold findPtrIdx at hfind
+  cases item with
+  | first =>
+    simp at hfind
+    cases hfind
+    omega
+  | last =>
+    simp at hfind
+    cases hfind
+    simp
+  | itemPtr item =>
+    simp at hfind
+    generalize heq : Array.findIdx? (fun i => decide (i = item)) arr = idx at hfind
+    cases idx with
+    | none =>
+      cases hfind
+    | some idx =>
+      cases hfind
+      rw [Array.findIdx?_eq_some_iff_findIdx_eq] at heq
+      obtain ⟨ _, _ ⟩ := heq
+      simp
+      omega
