LeanYjs/Algorithm/Invariant/Basic.lean
@@ -1,0 +1,291 @@
+import LeanYjs.Item
+import LeanYjs.ItemSet
+import LeanYjs.ClientId
+import LeanYjs.Order.ItemOrder
+import LeanYjs.Order.ItemSetInvariant
+import LeanYjs.Order.Totality
+import LeanYjs.Order.Transitivity
+import LeanYjs.Order.Asymmetry
+import LeanYjs.Algorithm.Insert.Basic
+import LeanYjs.Algorithm.Insert.Lemmas
+
+variable {A : Type}
+variable [DecidableEq A]
+
+def ArrSet (arr : List (YjsItem A)) : YjsPtr A -> Prop :=
+  fun a => match a with
+  | YjsPtr.itemPtr item => item ∈ arr
+  | YjsPtr.first => True
+  | YjsPtr.last => True
+
+def ArrSetClosed (arr : List (YjsItem A)) : Prop :=
+  IsClosedItemSet (ArrSet arr)
+
+omit [DecidableEq A] in theorem arr_set_closed_push (arr : List (YjsItem A)) (item : YjsItem A) :
+  ArrSetClosed arr ->
+  ArrSet arr item.origin ->
+  ArrSet arr item.rightOrigin ->
+  ArrSetClosed (item :: arr) := by
+  intros hclosed horigin hright
+  constructor
+  . simp [ArrSet]
+  . simp [ArrSet]
+  . intros o r id c d hor
+    cases o with
+    | itemPtr item' =>
+      simp [ArrSet] at hor
+      cases hor with
+      | inr hitem =>
+        right
+        apply hclosed.closedLeft at hitem
+        assumption
+      | inl heq =>
+        subst heq
+        right
+        assumption
+    | first =>
+      simp [ArrSet]
+    | last =>
+      simp [ArrSet]
+  . intros o r id c d hor
+    cases r with
+    | itemPtr item' =>
+      simp [ArrSet] at hor
+      cases hor with
+      | inr hitem =>
+        right
+        apply hclosed.closedRight at hitem
+        assumption
+      | inl heq =>
+        subst heq
+        right
+        assumption
+    | first =>
+      simp [ArrSet]
+    | last =>
+      simp [ArrSet]
+
+omit [DecidableEq A] in theorem arr_set_item_exists_index (arr arr' : List (YjsItem A)) (item : YjsItem A) :
+  ArrSetClosed arr' ->
+  ArrSet arr item ->
+  (∃ l, l ++ arr = arr') ->
+  ∃ i : Fin arr.length, arr[i] = item := by
+  intros hclosed hitem hsublist
+  induction arr with
+  | nil =>
+    simp [ArrSet] at hitem
+  | cons head arr ih =>
+    simp [ArrSet] at hitem
+    cases hitem with
+    | inl heq =>
+      subst heq
+      have zero_lt_len : 0 < (item :: arr).length := by simp
+      exists Fin.mk 0 zero_lt_len
+    | inr hin =>
+      have hsublist' : ∃ l', l' ++ arr = arr' := by
+        obtain ⟨ l, heq ⟩ := hsublist
+        exists (l ++ [head])
+        rw [List.append_assoc]
+        simp; assumption
+      obtain ⟨ i, hi ⟩ := ih hin hsublist'
+      let i' : Fin ((head :: arr).length) := by
+        simp
+        apply Fin.addNat i 1
+      exists i'
+
+omit [DecidableEq A] in theorem arr_set_closed_exists_index_for_origin :
+  ∀ (arr : List (YjsItem A)) (item : YjsItem A),
+  ArrSetClosed arr ->
+  ArrSet arr item ->
+  item.origin = YjsPtr.first ∨ item.origin = YjsPtr.last ∨ ∃ i : Fin arr.length, arr[i] = item.origin := by
+  intros arr item hclosed hitem
+  obtain ⟨ o, r, id, c, d ⟩ := item
+  apply hclosed.closedLeft at hitem
+  simp
+  cases o with
+  | first =>
+    left; simp
+  | last =>
+    right; left; simp
+  | itemPtr o =>
+    right; right
+    obtain ⟨ i, h ⟩ := arr_set_item_exists_index arr arr o hclosed hitem (by exists [])
+    exists i
+    simp
+    assumption
+
+omit [DecidableEq A] in theorem arr_set_closed_exists_index_for_right_origin :
+  ∀ (arr : List (YjsItem A)) (item : YjsItem A),
+  ArrSetClosed arr ->
+  ArrSet arr item ->
+  item.rightOrigin = YjsPtr.first ∨ item.rightOrigin = YjsPtr.last ∨ ∃ i : Fin arr.length, arr[i] = item.rightOrigin := by
+  intros arr item hclosed hitem
+  obtain ⟨ o, r, id, c, d ⟩ := item
+  apply hclosed.closedRight at hitem
+  simp
+  cases r with
+  | first =>
+    left; simp
+  | last =>
+    right; left; simp
+  | itemPtr o =>
+    right; right
+    obtain ⟨ i, h ⟩ := arr_set_item_exists_index arr arr o hclosed hitem (by exists [])
+    exists i
+    simp
+    assumption
+
+-- omit [DecidableEq A] in theorem yjs_lt_mono (P Q : ItemSet A) (x y : YjsPtr A) :
+--   IsClosedItemSet P ->
+--   ItemSetInvariant P ->
+--   (∀ a, P a -> Q a) ->
+--   YjsLt h x y ->
+--   YjsLt h x y := by
+--   intros hclosedP hinvP hsubset
+--   intros hlt
+--   revert hlt x y
+--   apply Nat.strongRec' (p := fun h => ∀ x y, YjsLt h x y → YjsLt h x y)
+--   intros n ih x y hlt
+--   cases hlt with
+--   | ltOriginOrder _  _ hlt =>
+--     apply YjsLt.ltOriginOrder
+--     . assumption
+--   | ltConflict _ _ _ hlt =>
+--     cases hlt with
+--     | ltOriginDiff =>
+--       apply YjsLt.ltConflict
+--       apply ConflictLt.ltOriginDiff
+--       all_goals (apply ih; unfold max4; omega)
+--       all_goals (assumption)
+--     | ltOriginSame =>
+--       apply YjsLt.ltConflict
+--       apply ConflictLt.ltOriginSame <;> try assumption
+--   | ltOrigin _ _ _ _ _ _ hlt =>
+--     apply YjsLt.ltOrigin
+--     . cases hlt with
+--       | leqSame =>
+--         apply YjsLeq.leqSame
+--       | leqLt =>
+--         apply YjsLeq.leqLt
+--         apply ih <;> try assumption
+--         omega
+--   | ltRightOrigin _ _ _ _ _ _ hlt =>
+--     apply YjsLt.ltRightOrigin
+--     . cases hlt with
+--       | leqSame =>
+--         apply YjsLeq.leqSame
+--       | leqLt =>
+--         apply YjsLeq.leqLt
+--         apply ih <;> try assumption
+--         omega
+
+-- omit [DecidableEq A] in theorem yjs_lt'_mono :
+--   ∀ (P Q : ItemSet A) (x y : YjsPtr A),
+--   IsClosedItemSet P ->
+--   ItemSetInvariant P ->
+--   (∀ a, P a -> Q a) ->
+--   YjsLt' x y -> YjsLt' x y := by
+--   intros P Q x y hclosedP hinvP hsubset hlt
+--   obtain ⟨ _, hlt ⟩ := hlt
+--   constructor
+--   apply yjs_lt_mono P Q x y hclosedP hinvP hsubset hlt
+
+-- omit [DecidableEq A] in theorem yjs_leq'_mono :
+--   ∀ (P Q : ItemSet A) (x y : YjsPtr A),
+--   IsClosedItemSet P ->
+--   ItemSetInvariant P ->
+--   (∀ a, P a -> Q a) ->
+--   YjsLeq' x y -> YjsLeq' x y := by
+--   intros P Q x y hclosedP hinvP hsubset hleq
+--   obtain ⟨ _, hleq ⟩ := hleq
+--   cases hleq with
+--   | leqSame =>
+--     exists 0
+--     apply YjsLeq.leqSame
+--   | leqLt =>
+--     constructor
+--     apply YjsLeq.leqLt
+--     apply yjs_lt_mono P Q x y hclosedP hinvP hsubset
+--     assumption
+
+theorem push_subset {A} (arr : List (YjsItem A)) (a : YjsItem A) :
+  ∀ x, ArrSet arr x -> ArrSet (a :: arr) x := by
+  intros x hin
+  unfold ArrSet at *
+  simp
+  cases x <;> (simp at *)
+  right; assumption
+
+theorem reachable_in {A} (arr : List (YjsItem A)) (a : YjsPtr A) :
+  IsClosedItemSet (ArrSet arr) ->
+  ∀ x, OriginReachable a x -> ArrSet arr a -> ArrSet arr x := by
+  intros hclosed x hreach hin
+  induction hreach with
+  | reachable_head x a y step h ih =>
+    cases step with
+    | reachable =>
+      simp [ArrSet] at hin
+      apply hclosed.closedLeft at hin
+      apply ih
+      assumption
+    | reachable_right =>
+      simp [ArrSet] at hin
+      apply hclosed.closedRight at hin
+      apply ih
+      assumption
+  | reachable_single _ _ hstep =>
+    cases hstep with
+    | reachable =>
+      simp [ArrSet] at hin
+      apply hclosed.closedLeft at hin
+      assumption
+    | reachable_right =>
+      simp [ArrSet] at hin
+      apply hclosed.closedRight at hin
+      assumption
+
+omit [DecidableEq A] in theorem item_set_invariant_push (arr : List (YjsItem A)) (item : YjsItem A) :
+  ItemSetInvariant (ArrSet arr) ->
+  ArrSetClosed arr ->
+  YjsLt' item.origin item.rightOrigin ->
+  (∀ x, OriginReachable item x -> YjsLeq' x item.origin ∨ YjsLeq' item.rightOrigin x) ->
+  (∀ x : YjsItem A, ArrSet arr x -> x.id = item.id -> x = item) ->
+  ItemSetInvariant (ArrSet (item :: arr)) := by
+  intros hinv hclosed horigin hreach hsameid
+  apply ItemSetInvariant.mk
+  . intros o r c id d hitem
+    simp [ArrSet] at hitem
+    cases hitem with
+    | inr hin =>
+      apply hinv.origin_not_leq at hin; assumption
+    | inl heq =>
+      subst heq
+      assumption
+  . intros o r c id d x hin
+    simp [ArrSet] at hin
+    cases hin with
+    | inr hin =>
+      apply hinv.origin_nearest_reachable _ _ _ _ _ _ hin
+    | inl heq =>
+      subst heq
+      simp at *
+      apply hreach _
+  . intros x y h_id_eq h_set_x h_set_y
+    simp [ArrSet] at *
+    cases h_set_x with
+    | inr hinx =>
+      cases h_set_y with
+      | inr hiny =>
+        apply hinv.id_unique _ _ h_id_eq hinx hiny
+      | inl hleq =>
+        subst hleq
+        apply hsameid _ hinx h_id_eq
+    | inl hinx =>
+      subst hinx
+      cases h_set_y with
+      | inr hiny =>
+        obtain h := hsameid y hiny (by rw [h_id_eq])
+        subst h; simp
+      | inl heqy =>
+        subst heqy
+        simp
