LeanYjs/Order/NoCrossOrigin.lean
@@ -26,7 +26,7 @@ theorem no_cross_origin {x y : YjsItem A} :
       x.size + y.size = hsize → YjsLeq' y.origin x.origin ∨ YjsLeq' (YjsPtr.itemPtr x) y.origin)
   intros n ih x y hpx hpy hlt hsize
   have hpy_origin : P y.origin := by
-    obtain ⟨ yo, yr, yid, yc ⟩ := y
+    obtain ⟨ yo, yr, yid, yc, yd ⟩ := y
     apply hP.closedLeft; assumption
   apply yjs_lt'_cases at hlt
   rcases hlt with
@@ -39,19 +39,19 @@ theorem no_cross_origin {x y : YjsItem A} :
   . cases heqlast
   . cases hx
     -- apply yjs_leq'_imp_eq_or_yjs_lt' at hleq'
-    obtain ⟨ xo, xr, xid, xc ⟩ := x
+    obtain ⟨ xo, xr, xid, xc, xd ⟩ := x
     have hpxo : P xo := by
       apply hP.closedLeft at hpx; assumption
     have hpxr : P xr := by
       apply hP.closedRight at hpx; assumption
     cases xr with
     | first =>
-      have ⟨ _, horlt ⟩ := hinv.origin_not_leq _ _ _ _ hpx
+      have ⟨ _, horlt ⟩ := hinv.origin_not_leq xo YjsPtr.first xc xid xd hpx
       apply not_ptr_lt_first hP hinv at horlt
       cases horlt
       apply hP.closedLeft at hpx; assumption
     | last =>
-      simp [YjsItem.rightOrigin] at hleq'
+      simp at hleq'
       have ⟨ _, hleq' ⟩ := hleq'
       cases hleq' with
       | leqLt h _ _ hlt' =>
@@ -60,20 +60,20 @@ theorem no_cross_origin {x y : YjsItem A} :
         assumption
     | itemPtr xr =>
       have hpxr_origin : P xr.origin := by
-        obtain ⟨ xro, xrr, xrid, xrc ⟩ := xr
+        obtain ⟨ xro, xrr, xrid, xrc, xrd ⟩ := xr
         apply hP.closedLeft; assumption
-      simp [YjsItem.rightOrigin] at hleq'
+      simp at hleq'
       apply yjs_leq'_imp_eq_or_yjs_lt' at hleq'
       cases hleq' with
       | inl hleq =>
         cases hleq
-        have hreachable : OriginReachable (YjsPtr.itemPtr (YjsItem.item xo (YjsPtr.itemPtr y) xid xc)) y.origin := by
+        have hreachable : OriginReachable (YjsPtr.itemPtr (YjsItem.mk xo (YjsPtr.itemPtr y) xid xc xd)) y.origin := by
           apply OriginReachable.reachable_head (y := YjsPtr.itemPtr y)
           . apply OriginReachableStep.reachable_right
-          . obtain ⟨ yo, yr, yid, yc ⟩ := y
+          . obtain ⟨ yo, yr, yid, yc, yd ⟩ := y
             apply OriginReachable.reachable_single
             apply OriginReachableStep.reachable
-        cases hinv.origin_nearest_reachable (x := y.origin) _ _ _ _ hpx hreachable with
+        cases hinv.origin_nearest_reachable xo (YjsPtr.itemPtr y) xc xid xd y.origin hpx hreachable with
         | inl hleq =>
           left
           assumption
@@ -82,14 +82,14 @@ theorem no_cross_origin {x y : YjsItem A} :
           cases hleq with
           | inr hlt =>
             have hltorigin : YjsLt' y.origin y := by
-              obtain ⟨ yo, yr, yid, yc ⟩ := y
+              obtain ⟨ yo, yr, yid, yc, yd ⟩ := y
               constructor; apply YjsLt.ltOrigin <;> try assumption
               apply YjsLeq.leqSame
             by_contra
             apply yjs_lt_asymm hP hinv y.origin y hpy_origin hpy hltorigin hlt
           | inl heq =>
-            obtain ⟨ yo, yr, yid, yc ⟩ := y
-            simp [YjsItem.origin] at heq
+            obtain ⟨ yo, yr, yid, yc, yd ⟩ := y
+            simp at heq
             cases heq
       | inr hlt =>
         have hsize' : xr.size + y.size < n := by
@@ -101,26 +101,26 @@ theorem no_cross_origin {x y : YjsItem A} :
         | inl hleq =>
           obtain ⟨ h, hleq ⟩ := hleq
           left
-          have hreachable : OriginReachable (YjsPtr.itemPtr (YjsItem.item xo xr xid xc)) xr.origin := by
+          have hreachable : OriginReachable (YjsPtr.itemPtr (YjsItem.mk xo xr xid xc xd)) xr.origin := by
             apply OriginReachable.reachable_head
             apply OriginReachableStep.reachable_right
             . apply OriginReachable.reachable_single
-              obtain ⟨ xro, xrr, xrid, xrc ⟩ := xr
+              obtain ⟨ xro, xrr, xrid, xrc, xrd ⟩ := xr
               apply OriginReachableStep.reachable
           have ⟨ _, hlt ⟩ : YjsLeq' xr.origin xo := by
-            cases hinv.origin_nearest_reachable _ _ _ _ _ hpx hreachable with
+            cases hinv.origin_nearest_reachable xo xr xc xid xd xr.origin hpx hreachable with
             | inl hleq => assumption
             | inr hleq =>
               have hlt : YjsLt' xr.origin xr := by
-                obtain ⟨ xro, xrr, xrid, xrc ⟩ := xr
+                obtain ⟨ xro, xrr, xrid, xrc, xrd ⟩ := xr
                 constructor; apply YjsLt.ltOrigin <;> try assumption
                 . apply YjsLeq.leqSame
               apply yjs_leq'_imp_eq_or_yjs_lt' at hleq
               cases hleq with
               | inl heq =>
                 by_contra
-                obtain ⟨ xro, xrr, xrid, xrc ⟩ := xr
-                simp [YjsItem.origin] at *
+                obtain ⟨ xro, xrr, xrid, xrc, xrd ⟩ := xr
+                simp at *
                 cases heq
               | inr hlt' =>
                 cases yjs_lt_asymm hP hinv _ _ hpxr_origin hpxr hlt hlt'
@@ -129,7 +129,7 @@ theorem no_cross_origin {x y : YjsItem A} :
         | inr hlt =>
           obtain ⟨ _, hlt ⟩ := hlt
           right
-          have ⟨ h', hlt' ⟩ : YjsLt' (YjsPtr.itemPtr (YjsItem.item xo (YjsPtr.itemPtr xr) xid xc)) xr := by
+          have ⟨ h', hlt' ⟩ : YjsLt' (YjsPtr.itemPtr (YjsItem.mk xo (YjsPtr.itemPtr xr) xid xc xd)) xr := by
             constructor; apply YjsLt.ltRightOrigin <;> try assumption
             . apply YjsLeq.leqSame
           apply yjs_leq_p_trans (h1 := h' + 1) (inv := hinv) (y := xr) <;> try assumption
